Add gadget that removes immediately forced thunks

compiler/backend/proofs/thunk_caseProofScript.sml
@@ -731,10 +731,6 @@ Inductive exp_rel_d2b:
        v_rel_d2b (Thunk (INL v)) (Thunk (INL w)))
 End
 
-Theorem SUM_REL_def[local,simp] = quotient_sumTheory.SUM_REL_def;
-
-Theorem PAIR_REL_def[local,simp] = quotient_pairTheory.PAIR_REL;
-
 Theorem v_rel_d2b_cases[local] = CONJUNCT2 exp_rel_d2b_cases;
 
 (* Boilerplate *)
@@ -1812,10 +1808,6 @@ Inductive exp_rel_inl:
        v_rel_inl (Thunk (INL v)) (Thunk (INL w)))
 End
 
-Theorem SUM_REL_def[local,simp] = quotient_sumTheory.SUM_REL_def;
-
-Theorem PAIR_REL_def[local,simp] = quotient_pairTheory.PAIR_REL;
-
 Theorem v_rel_inl_cases[local] = CONJUNCT2 exp_rel_inl_cases;
 
 Theorem v_rel_inl_def[simp] =
@@ -2442,6 +2434,528 @@ Proof
       \\ rw []
       \\ first_x_assum (drule_then assume_tac)
       \\ first_x_assum (drule_all_then assume_tac)
+      \\ first_x_assum (drule_all_then assume_tac)
+      \\ rpt CASE_TAC \\ gs []))
+QED
+
+(* -------------------------------------------------------------------------
+ * exp_rel_unbox:
+ *
+ * Remove immediately forced thunks introduced by exp_rel_inl.
+ * ------------------------------------------------------------------------- *)
+
+Inductive exp_rel_unbox:
+(* Force replacement *)
+[exp_rel_unbox_Unbox:]
+  (∀v.
+     exp_rel_unbox (Force (Box (Var v))) (Tick (Var v))) ∧
+[exp_rel_unbox_Unbox_Value:]
+  (∀v w.
+     v_rel_unbox v w ⇒
+       exp_rel_unbox (Force (Box (Value v))) (Tick (Value w))) ∧
+(* Boilerplate: *)
+[exp_rel_unbox_App:]
+  (∀f g x y.
+     exp_rel_unbox f g ∧
+     exp_rel_unbox x y ⇒
+       exp_rel_unbox (App f x) (App g y)) ∧
+[exp_rel_unbox_Lam:]
+  (∀s x y.
+     exp_rel_unbox x y ⇒
+       exp_rel_unbox (Lam s x) (Lam s y)) ∧
+[exp_rel_unbox_Letrec:]
+  (∀f g x y.
+     LIST_REL (λ(fn,x) (gn,y).
+                 fn = gn ∧
+                 ok_binder x ∧
+                 exp_rel_unbox x y) f g ∧
+     exp_rel_unbox x y ⇒
+       exp_rel_unbox (Letrec f x) (Letrec g y)) ∧
+[exp_rel_unbox_Let:]
+  (∀b x1 y1 x2 y2.
+     exp_rel_unbox x1 x2 ∧
+     exp_rel_unbox y1 y2 ⇒
+       exp_rel_unbox (Let b x1 y1) (Let b x2 y2)) ∧
+[exp_rel_unbox_If:]
+  (∀x1 x2 y1 y2 z1 z2.
+     LIST_REL exp_rel_unbox [x1;y1;z1] [x2;y2;z2] ⇒
+       exp_rel_unbox (If x1 y1 z1) (If x2 y2 z2)) ∧
+[exp_rel_unbox_Prim:]
+  (∀op xs ys.
+     LIST_REL exp_rel_unbox xs ys ⇒
+       exp_rel_unbox (Prim op xs) (Prim op ys)) ∧
+[exp_rel_unbox_Delay:]
+  (∀x y.
+     exp_rel_unbox x y ⇒
+       exp_rel_unbox (Delay x) (Delay y)) ∧
+[exp_rel_unbox_Box:]
+  (∀x y.
+     exp_rel_unbox x y ⇒
+       exp_rel_unbox (Box x) (Box y)) ∧
+[exp_rel_unbox_Force:]
+  (∀x y.
+     exp_rel_unbox x y ⇒
+       exp_rel_unbox (Force x) (Force y)) ∧
+[exp_rel_unbox_MkTick:]
+  (∀x y.
+     exp_rel_unbox x y ⇒
+       exp_rel_unbox (MkTick x) (MkTick y)) ∧
+[exp_rel_unbox_Var:]
+  (∀v.
+     exp_rel_unbox (Var v) (Var v)) ∧
+[exp_rel_unbox_Value:]
+  (∀v w.
+     v_rel_unbox v w ⇒
+       exp_rel_unbox (Value v) (Value w)) ∧
+[v_rel_unbox_Atom:]
+  (∀x.
+     v_rel_unbox (Atom x) (Atom x)) ∧
+[v_rel_unbox_Constructor:]
+  (∀vs ws.
+     LIST_REL v_rel_unbox vs ws ⇒
+       v_rel_unbox (Constructor s vs) (Constructor s ws)) ∧
+[v_rel_unbox_Closure:]
+  (∀s x y.
+     exp_rel_unbox x y ⇒
+       v_rel_unbox (Closure s x) (Closure s y)) ∧
+[v_rel_unbox_DoTick:]
+  (∀v w.
+     v_rel_unbox v w ⇒
+       v_rel_unbox (DoTick v) (DoTick w)) ∧
+[v_rel_unbox_Recclosure:]
+  (∀f g n.
+     LIST_REL (λ(fn,x) (gn,y).
+                 fn = gn ∧
+                 ok_binder x ∧
+                 exp_rel_unbox x y) f g ⇒
+       v_rel_unbox (Recclosure f n) (Recclosure g n)) ∧
+[v_rel_unbox_Thunk_INR:]
+  (∀x y.
+     exp_rel_unbox x y ⇒
+       v_rel_unbox (Thunk (INR x)) (Thunk (INR y))) ∧
+[v_rel_unbox_Thunk_INL:]
+  (∀v w.
+     v_rel_unbox v w ⇒
+       v_rel_unbox (Thunk (INL v)) (Thunk (INL w)))
+End
+
+Theorem v_rel_unbox_cases[local] = CONJUNCT2 exp_rel_unbox_cases;
+
+Theorem v_rel_unbox_def[simp] =
+  [ “v_rel_unbox (Closure s x) z”,
+    “v_rel_unbox z (Closure s x)”,
+    “v_rel_unbox (Recclosure s x) z”,
+    “v_rel_unbox z (Recclosure s x)”,
+    “v_rel_unbox (Constructor s x) z”,
+    “v_rel_unbox z (Constructor s x)”,
+    “v_rel_unbox (Atom s) z”,
+    “v_rel_unbox z (Atom s)”,
+    “v_rel_unbox (Thunk (INL s)) z”,
+    “v_rel_unbox z (Thunk (INL s))”,
+    “v_rel_unbox (Thunk (INR s)) z”,
+    “v_rel_unbox z (Thunk (INR s))” ]
+  |> map (SIMP_CONV (srw_ss ()) [Once v_rel_unbox_cases])
+  |> LIST_CONJ;
+
+Theorem exp_rel_unbox_subst:
+  ∀vs x ws y.
+    MAP FST vs = MAP FST ws ∧
+    LIST_REL v_rel_unbox (MAP SND vs) (MAP SND ws) ∧
+    exp_rel_unbox x y ⇒
+      exp_rel_unbox (subst vs x) (subst ws y)
+Proof
+  ho_match_mp_tac subst_ind \\ rw []
+  \\ qpat_x_assum ‘exp_rel_unbox _ _’ mp_tac
+  >- ((* Var *)
+    rw [Once exp_rel_unbox_cases]
+    \\ simp [subst_def]
+    \\ ‘OPTREL v_rel_unbox (ALOOKUP (REVERSE vs) s) (ALOOKUP (REVERSE ws) s)’
+      suffices_by (
+        strip_tac
+        \\ gs [OPTREL_def, exp_rel_unbox_Var, exp_rel_unbox_Value])
+    \\ irule LIST_REL_OPTREL
+    \\ gs [LIST_REL_CONJ, ELIM_UNCURRY, EVERY2_MAP]
+    \\ last_x_assum mp_tac
+    \\ pop_assum kall_tac
+    \\ qid_spec_tac ‘ws’
+    \\ Induct_on ‘vs’ \\ simp []
+    \\ Cases_on ‘ws’ \\ simp [])
+  >- ((* Prim *)
+    rw [Once exp_rel_unbox_cases] \\ gs []
+    \\ simp [subst_def]
+    \\ irule exp_rel_unbox_Prim
+    \\ gs [EVERY2_MAP, EVERY2_refl_EQ]
+    \\ irule LIST_REL_mono
+    \\ first_assum (irule_at Any) \\ gs [])
+  >- ((* If *)
+    rw [Once exp_rel_unbox_cases]
+    \\ simp [subst_def]
+    \\ irule exp_rel_unbox_If \\ fs [])
+  >- ((* App *)
+    rw [Once exp_rel_unbox_cases]
+    \\ simp [subst_def]
+    \\ irule exp_rel_unbox_App \\ fs [])
+  >- ((* Lam *)
+    rw [Once exp_rel_unbox_cases]
+    \\ gs [subst_def]
+    \\ irule exp_rel_unbox_Lam
+    \\ first_x_assum irule
+    \\ gs [MAP_FST_FILTER, EVERY2_MAP]
+    \\ qabbrev_tac ‘P = λn. n ≠ s’ \\ gs []
+    \\ irule LIST_REL_FILTER \\ gs []
+    \\ irule LIST_REL_mono
+    \\ first_x_assum (irule_at Any)
+    \\ simp [FORALL_PROD])
+  >- ((* Let NONE *)
+    rw [Once exp_rel_unbox_cases]
+    \\ gs [subst_def]
+    \\ irule exp_rel_unbox_Let \\ fs [])
+  >- ((* Let SOME *)
+    rw [Once exp_rel_unbox_cases] \\ gs []
+    \\ gs [subst_def]
+    \\ irule exp_rel_unbox_Let \\ gs []
+    \\ first_x_assum irule
+    \\ gs [MAP_FST_FILTER, EVERY2_MAP]
+    \\ qabbrev_tac ‘P = λn. n ≠ s’ \\ gs []
+    \\ irule LIST_REL_FILTER \\ gs []
+    \\ irule LIST_REL_mono
+    \\ first_x_assum (irule_at Any)
+    \\ simp [FORALL_PROD])
+  >- ((* Letrec *)
+    rw [Once exp_rel_unbox_cases] \\ gs []
+    \\ simp [subst_def]
+    \\ irule exp_rel_unbox_Letrec
+    \\ gvs [EVERY2_MAP, LAMBDA_PROD]
+    \\ simp [MAP_MAP_o, combinTheory.o_DEF, LAMBDA_PROD, GSYM FST_THM]
+    \\ first_x_assum (irule_at Any)
+    \\ `MAP FST f = MAP FST g`
+      by (irule LIST_EQ
+          \\ gvs [EL_MAP, LIST_REL_EL_EQN, ELIM_UNCURRY])
+    \\ qabbrev_tac ‘P = λx. ¬MEM x (MAP FST g)’ \\ fs []
+    \\ gvs [MAP_FST_FILTER, EVERY2_MAP]
+    \\ irule_at Any LIST_REL_FILTER
+    \\ irule_at Any LIST_REL_mono
+    \\ first_assum (irule_at Any)
+    \\ simp [FORALL_PROD]
+    \\ irule LIST_REL_mono
+    \\ first_assum (irule_at Any)
+    \\ simp [FORALL_PROD] \\ rw []
+    \\ first_x_assum irule
+    \\ simp [MAP_FST_FILTER, SF SFY_ss]
+    \\ irule LIST_REL_FILTER \\ gs []
+    \\ irule LIST_REL_mono
+    \\ first_assum (irule_at Any)
+    \\ simp [FORALL_PROD])
+  >- ((* Delay *)
+    rw [Once exp_rel_unbox_cases]
+    \\ simp [subst_def]
+    \\ irule exp_rel_unbox_Delay \\ gs [])
+  >- ((* Box *)
+    rw [Once exp_rel_unbox_cases] \\ gs []
+    \\ simp [subst_def]
+    \\ irule exp_rel_unbox_Box \\ gs [])
+  >- ((* Force *)
+    rw [Once exp_rel_unbox_cases]
+    \\ simp [subst_def, FILTER_T, ELIM_UNCURRY, exp_rel_unbox_Force,
+             exp_rel_unbox_Unbox_Value]
+    \\ ‘OPTREL v_rel_unbox (ALOOKUP (REVERSE vs) v) (ALOOKUP (REVERSE ws) v)’
+      suffices_by (
+        strip_tac
+        \\ gs [OPTREL_def, exp_rel_unbox_Var, exp_rel_unbox_Unbox,
+               exp_rel_unbox_Unbox_Value])
+    \\ irule LIST_REL_OPTREL
+    \\ gs [LIST_REL_CONJ, ELIM_UNCURRY, EVERY2_MAP]
+    \\ qpat_x_assum ‘MAP FST vs = _’ mp_tac
+    \\ rpt (pop_assum kall_tac)
+    \\ qid_spec_tac ‘ws’
+    \\ Induct_on ‘vs’ \\ simp []
+    \\ Cases_on ‘ws’ \\ simp [])
+  >- ((* Value *)
+    rw [Once exp_rel_unbox_cases]
+    \\ simp [subst_def, exp_rel_unbox_Value])
+  >- ((* MkTick *)
+    rw [Once exp_rel_unbox_cases]
+    \\ simp [subst_def]
+    \\ irule exp_rel_unbox_MkTick \\ gs [])
+QED
+
+Theorem exp_rel_unbox_eval_to:
+  ∀k x y m.
+    exp_rel_unbox x y ⇒
+      ($= +++ v_rel_unbox)
+        (eval_to k x)
+        (eval_to k y)
+Proof
+  ho_match_mp_tac eval_to_ind \\ simp []
+  \\ rpt conj_tac \\ rpt gen_tac
+  >~ [‘Var v’] >- (
+    rw [Once exp_rel_unbox_cases]
+    \\ simp [eval_to_def])
+  >~ [‘Value v’] >- (
+    rw [Once exp_rel_unbox_cases]
+    \\ simp [eval_to_def])
+  >~ [‘App f x’] >- (
+    strip_tac
+    \\ rw [Once exp_rel_unbox_cases] \\ gs []
+    \\ rename1 ‘exp_rel_unbox x y’
+    \\ gs [eval_to_def]
+    \\ first_x_assum (drule_all_then assume_tac)
+    \\ first_x_assum (drule_all_then assume_tac)
+    \\ Cases_on ‘eval_to k f’ \\ Cases_on ‘eval_to k g’ \\ gvs []
+    \\ rename1 ‘v_rel_unbox v w’
+    \\ Cases_on ‘eval_to k x’ \\ Cases_on ‘eval_to k y’ \\ gs []
+    \\ Cases_on ‘v’ \\ Cases_on ‘w’ \\ gvs [dest_anyClosure_def]
+    >- ((* Closure *)
+      IF_CASES_TAC \\ gs []
+      \\ rename1 ‘(_ +++ _) (_ _ (subst1 s u1 e1)) (_ _ (subst1 s u2 e2))’
+      \\ ‘[s,u1] = [] ++ [s,u1]’ by gs [] \\ pop_assum SUBST1_TAC
+      \\ ‘[s,u2] = [] ++ [s,u2]’ by gs [] \\ pop_assum SUBST1_TAC
+      \\ first_x_assum irule \\ gs [closed_subst]
+      \\ irule_at Any exp_rel_unbox_subst
+      \\ first_assum (irule_at Any) \\ gs [])
+        (* Recclosure *)
+    \\ rename1 ‘LIST_REL _ xs ys’
+    \\ ‘OPTREL exp_rel_unbox (ALOOKUP (REVERSE xs) s)
+                             (ALOOKUP (REVERSE ys) s)’
+      by (irule LIST_REL_OPTREL \\ gs []
+          \\ gs [ELIM_UNCURRY, LIST_REL_CONJ])
+    \\ gs [OPTREL_def]
+    \\ gvs [Once exp_rel_unbox_cases]
+    \\ IF_CASES_TAC \\ gs []
+    \\ first_x_assum irule
+    \\ irule_at Any exp_rel_unbox_subst
+    \\ first_assum (irule_at Any)
+    \\ simp [EVERY2_MAP, LAMBDA_PROD]
+    \\ irule_at Any LIST_REL_mono
+    \\ first_assum (irule_at Any)
+    \\ csimp [FORALL_PROD]
+    \\ simp [closed_subst, MAP_MAP_o, combinTheory.o_DEF, LAMBDA_PROD, GSYM
+             FST_THM]
+    \\ irule_at Any LIST_EQ
+    \\ gvs [LIST_REL_EL_EQN, EL_MAP, ELIM_UNCURRY])
+  >~ [‘Lam s x’] >- (
+    rw [Once exp_rel_unbox_cases]
+    \\ gs [eval_to_def, v_rel_unbox_def])
+  >~ [‘Let NONE x y’] >- (
+    strip_tac
+    \\ rw [Once exp_rel_unbox_cases] \\ gs []
+    \\ simp [eval_to_def]
+    \\ IF_CASES_TAC \\ gs []
+    \\ last_x_assum (drule_all_then assume_tac)
+    \\ Cases_on ‘eval_to (k - 1) x’ \\ Cases_on ‘eval_to (k - 1) x2’ \\ gs [])
+  >~ [‘Let (SOME n) x y’] >- (
+    strip_tac
+    \\ rw [Once exp_rel_unbox_cases] \\ gs []
+    \\ simp [eval_to_def]
+    \\ IF_CASES_TAC \\ gs []
+    \\ first_x_assum (drule_then assume_tac)
+    \\ Cases_on ‘eval_to (k - 1) x’ \\ Cases_on ‘eval_to (k - 1) x2’ \\ gs []
+    \\ first_x_assum irule
+    \\ irule_at Any exp_rel_unbox_subst \\ gs [])
+  >~ [‘Letrec f x’] >- (
+    strip_tac
+    \\ rw [Once exp_rel_unbox_cases] \\ gs []
+    \\ simp [eval_to_def]
+    \\ IF_CASES_TAC \\ gs []
+    \\ first_x_assum irule
+    \\ simp [subst_funs_def, closed_subst, MAP_MAP_o, combinTheory.o_DEF,
+             LAMBDA_PROD, GSYM FST_THM]
+    \\ irule_at Any exp_rel_unbox_subst
+    \\ simp [subst_funs_def, closed_subst, MAP_MAP_o, combinTheory.o_DEF,
+             LAMBDA_PROD, GSYM FST_THM, EVERY2_MAP]
+    \\ irule_at Any LIST_EQ
+    \\ gvs [LIST_REL_EL_EQN, EL_MAP, ELIM_UNCURRY])
+  >~ [‘If x1 y1 z1’] >- (
+    strip_tac
+    \\ rw [Once exp_rel_unbox_cases] \\ gs []
+    \\ simp [eval_to_def]
+    \\ IF_CASES_TAC \\ gs []
+    \\ first_x_assum (drule_all_then assume_tac)
+    \\ first_x_assum (drule_all_then assume_tac)
+    \\ first_x_assum (drule_all_then assume_tac)
+    \\ Cases_on ‘eval_to (k - 1) x1’ \\ Cases_on ‘eval_to (k - 1) x2’ \\ gs []
+    \\ IF_CASES_TAC \\ gs []
+    \\ IF_CASES_TAC \\ gs []
+    \\ IF_CASES_TAC \\ gs []
+    \\ IF_CASES_TAC \\ gs [])
+  >~ [‘Force x’] >- (
+    strip_tac
+    \\ rw [Once exp_rel_unbox_cases] \\ gs []
+    >- (
+      once_rewrite_tac [eval_to_def]
+      \\ IF_CASES_TAC \\ gs []
+      \\ simp [Once eval_to_def]
+      \\ simp [Once eval_to_def]
+      \\ simp [subst_funs_def, eval_to_def])
+    >- ((* Unbox *)
+      once_rewrite_tac [eval_to_def]
+      \\ IF_CASES_TAC \\ gs []
+      \\ simp [Once eval_to_def, subst_funs_def]
+      \\ once_rewrite_tac [eval_to_def]
+      \\ simp [dest_anyThunk_def])
+    \\ rename1 ‘exp_rel_unbox x y’
+    \\ CONV_TAC (LAND_CONV (SIMP_CONV (srw_ss()) [Once eval_to_def]))
+    \\ CONV_TAC (RAND_CONV (SIMP_CONV (srw_ss()) [Once eval_to_def]))
+    \\ IF_CASES_TAC \\ gs []
+    \\ first_x_assum (drule_all_then assume_tac)
+    \\ Cases_on ‘eval_to k x’ \\ Cases_on ‘eval_to k y’ \\ gs []
+    \\ rename1 ‘v_rel_unbox v w’
+    \\ Cases_on ‘dest_Tick v’ \\ gs []
+    >- (
+      ‘dest_Tick w = NONE’
+        by (Cases_on ‘v’ \\ Cases_on ‘w’ \\ gs []
+            \\ gs [Once v_rel_unbox_cases])
+      \\ gs []
+      \\ Cases_on ‘v’ \\ Cases_on ‘w’ \\ gvs [dest_anyThunk_def]
+      >- (
+        rename1 ‘LIST_REL _ xs ys’
+        \\ ‘OPTREL (λx0 y0. ok_binder x0 ∧
+                            exp_rel_unbox x0 y0)
+                   (ALOOKUP (REVERSE xs) s)
+                   (ALOOKUP (REVERSE ys) s)’
+          by (irule LIST_REL_OPTREL \\ gs []
+              \\ gs [ELIM_UNCURRY, LIST_REL_CONJ])
+        \\ gs [OPTREL_def]
+        \\ gvs [Once exp_rel_unbox_cases]
+        \\ first_x_assum irule
+        \\ simp [subst_funs_def]
+        \\ irule_at Any exp_rel_unbox_subst
+        \\ gs [MAP_MAP_o, combinTheory.o_DEF, EVERY2_MAP, LAMBDA_PROD,
+               GSYM FST_THM]
+        \\ irule_at Any LIST_REL_mono
+        \\ csimp [FORALL_PROD]
+        \\ first_assum (irule_at Any)
+        \\ simp []
+        \\ irule LIST_EQ
+        \\ gvs [LIST_REL_EL_EQN, EL_MAP, ELIM_UNCURRY])
+      \\ CASE_TAC \\ gs []
+      \\ first_x_assum irule
+      \\ simp [subst_funs_def, SF SFY_ss])
+    \\ ‘∃y. dest_Tick w = SOME y’
+        by (Cases_on ‘v’ \\ Cases_on ‘w’ \\ gs []
+            \\ gs [Once v_rel_unbox_cases])
+    \\ gs []
+    \\ first_x_assum irule
+    \\ rw [Once exp_rel_unbox_cases]
+    \\ rw [Once exp_rel_unbox_cases]
+    \\ Cases_on ‘v’ \\ Cases_on ‘w’ \\ gs [Once v_rel_unbox_cases])
+  >~ [‘Delay x’] >- (
+    rw [Once exp_rel_unbox_cases] \\ gs []
+    \\ simp [eval_to_def])
+  >~ [‘Box x’] >- (
+    strip_tac
+    \\ rw [Once exp_rel_unbox_cases] \\ gs []
+    \\ simp [eval_to_def]
+    \\ rename1 ‘exp_rel_unbox x y’
+    \\ first_x_assum (drule_then assume_tac)
+    \\ Cases_on ‘eval_to k x’ \\ Cases_on ‘eval_to k y’ \\ gs [])
+  >~ [‘MkTick x’] >- (
+    strip_tac
+    \\ rw [Once exp_rel_unbox_cases] \\ gs []
+    \\ simp [eval_to_def]
+    \\ rename1 ‘exp_rel_unbox x y’
+    \\ first_x_assum (drule_all_then assume_tac)
+    \\ Cases_on ‘eval_to k x’ \\ Cases_on ‘eval_to k y’ \\ gs []
+    \\ rw [Once v_rel_unbox_cases])
+  >~ [‘Prim op xs’] >- (
+    strip_tac
+    \\ rw [Once exp_rel_unbox_cases] \\ gs []
+    \\ simp [eval_to_def]
+    \\ Cases_on ‘op’ \\ gs [EVERY_EL]
+    >- ((* Cons *)
+      gs [result_map_def, MEM_MAP, PULL_EXISTS, LIST_REL_EL_EQN, MEM_EL]
+      \\ IF_CASES_TAC \\ gs []
+      >- (
+        gvs [MEM_EL, PULL_EXISTS, LIST_REL_EL_EQN]
+        \\ first_x_assum (drule_then assume_tac) \\ gs []
+        \\ first_x_assum (drule_then assume_tac) \\ gs []
+        \\ first_x_assum (drule_all_then assume_tac) \\ gs []
+        \\ Cases_on ‘eval_to k (EL n ys)’ \\ gvs []
+        \\ rw [] \\ gs [])
+      \\ gs [Once (DECIDE “A ⇒ ¬B ⇔ B ⇒ ¬A”)]
+      \\ IF_CASES_TAC \\ gs []
+      >- (
+        IF_CASES_TAC \\ gs []
+        >- (
+          rename1 ‘j < LENGTH ys’
+          \\ first_x_assum (drule_then assume_tac)
+          \\ first_x_assum (drule_then assume_tac)
+          \\ first_x_assum (drule_all_then assume_tac)
+          \\ Cases_on ‘eval_to k (EL j xs)’ \\ gs [])
+        \\ gs [Once (DECIDE “A ⇒ ¬B ⇔ B ⇒ ¬A”)]
+        \\ rw [] \\ gs []
+        \\ gs [Once (DECIDE “A ⇒ ¬B ⇔ B ⇒ ¬A”)]
+        \\ first_x_assum (drule_then assume_tac) \\ gs []
+        \\ first_x_assum (drule_then assume_tac) \\ gs []
+        \\ first_x_assum (drule_all_then assume_tac) \\ gs []
+        \\ first_x_assum (drule_all_then assume_tac) \\ gs []
+        \\ Cases_on ‘eval_to k (EL n ys)’ \\ gs [])
+      \\ gs [Once (DECIDE “A ⇒ ¬B ⇔ B ⇒ ¬A”)]
+      \\ IF_CASES_TAC \\ gs []
+      >- (
+        first_x_assum (drule_then assume_tac)
+        \\ first_x_assum (drule_then assume_tac)
+        \\ first_x_assum (drule_then assume_tac)
+        \\ first_x_assum (drule_all_then assume_tac)
+        \\ Cases_on ‘eval_to k (EL n xs)’ \\ gs [])
+      \\ gs [Once (DECIDE “A ⇒ ¬B ⇔ B ⇒ ¬A”)]
+      \\ IF_CASES_TAC \\ gs []
+      >- (
+        first_x_assum (drule_then assume_tac)
+        \\ first_x_assum (drule_then assume_tac)
+        \\ first_x_assum (drule_then assume_tac)
+        \\ first_x_assum (drule_all_then assume_tac)
+        \\ first_x_assum (drule_all_then assume_tac)
+        \\ Cases_on ‘eval_to k (EL n xs)’ \\ gs [])
+      \\ gs [Once (DECIDE “A ⇒ ¬B ⇔ B ⇒ ¬A”)]
+      \\ rw [EVERY2_MAP, LIST_REL_EL_EQN]
+      \\ first_x_assum (drule_then assume_tac)
+      \\ first_x_assum (drule_then assume_tac)
+      \\ first_x_assum (drule_then assume_tac)
+      \\ first_x_assum (drule_then assume_tac)
+      \\ first_x_assum (drule_then assume_tac)
+      \\ first_x_assum (drule_all_then assume_tac)
+      \\ Cases_on ‘eval_to k (EL n xs)’
+      \\ Cases_on ‘eval_to k (EL n ys)’ \\ gs []
+      \\ rename1 ‘err ≠ Type_error’ \\ Cases_on ‘err’ \\ gs [])
+    >- ((* IsEq *)
+      gvs [LIST_REL_EL_EQN]
+      \\ IF_CASES_TAC \\ gs []
+      \\ gvs [LENGTH_EQ_NUM_compute, DECIDE “n < 1n ⇔ n = 0”]
+      \\ IF_CASES_TAC \\ gs []
+      \\ rename1 ‘exp_rel_unbox x y’
+      \\ first_x_assum (drule_then assume_tac)
+      \\ Cases_on ‘eval_to (k - 1) x’ \\ Cases_on ‘eval_to (k - 1) y’ \\ gs []
+      \\ rename1 ‘v_rel_unbox v w’
+      \\ Cases_on ‘v’ \\ Cases_on ‘w’ \\ gvs [LIST_REL_EL_EQN]
+      \\ IF_CASES_TAC \\ gs [])
+    >- ((* Proj *)
+      gvs [LIST_REL_EL_EQN]
+      \\ IF_CASES_TAC \\ gs []
+      \\ gvs [LENGTH_EQ_NUM_compute, DECIDE “n < 1n ⇔ n = 0”]
+      \\ IF_CASES_TAC \\ gs []
+      \\ rename1 ‘exp_rel_unbox x y’
+      \\ first_x_assum (drule_then assume_tac)
+      \\ Cases_on ‘eval_to (k - 1) x’ \\ Cases_on ‘eval_to (k - 1) y’ \\ gs []
+      \\ rename1 ‘v_rel_unbox v w’
+      \\ Cases_on ‘v’ \\ Cases_on ‘w’ \\ gvs [LIST_REL_EL_EQN]
+      \\ IF_CASES_TAC \\ gs [])
+    >- ((* AtomOp *)
+      qmatch_goalsub_abbrev_tac ‘result_map f xs’
+      \\ qmatch_goalsub_abbrev_tac ‘result_map g ys’
+      \\ ‘MAP f xs = MAP g ys’
+        suffices_by (
+          rw []
+          \\ simp [result_map_def]
+          \\ IF_CASES_TAC \\ gs []
+          \\ IF_CASES_TAC \\ gs []
+          \\ CASE_TAC \\ gs []
+          \\ CASE_TAC \\ gs [])
+      \\ unabbrev_all_tac
+      \\ irule LIST_EQ
+      \\ gvs [LIST_REL_EL_EQN, MEM_EL, PULL_EXISTS, EL_MAP]
+      \\ rw []
+      \\ first_x_assum (drule_then assume_tac)
       \\ first_x_assum (drule_all_then assume_tac)
       \\ rpt CASE_TAC \\ gs []))
 QED
